Isabelle/01_Core/Range_p.thy
@@ -1,0 +1,18 @@
+theory Range_p
+  imports Definitions Equalities
+begin
+section \<open>Range_p properties for top\<close>
+
+lemma same_range_p_3: "p\<^sub>1 \<equiv>\<^sub>p p\<^sub>2 \<Longrightarrow> Range_p p\<^sub>1 = Range_p p\<^sub>2"
+  by (auto simp: Range_p_def equiv_def restr_post_def)
+
+theorem same_range_p_2: "a \<triangleq> b \<Longrightarrow> Range_p a = Range_p b"
+  using inverse_equality_1 same_range_p_3 by blast
+
+theorem range_p_explicit_1: "y \<in> Range_p a \<Longrightarrow> \<exists>x. (x,y) \<in> post a \<and> x \<in> Pre a"
+  by (auto simp: Range_p_def restrict_r_def)
+
+theorem range_p_explicit_2: "(x,y) \<in> post a \<and> x \<in> Pre a \<Longrightarrow> y \<in> Range_p a"
+  by (auto simp: Range_p_def restrict_r_def)
+
+end
