Isabelle/02_Fundamental_operations/Corestriction.thy
@@ -1,82 +1,93 @@
 theory Corestriction
   imports "../T_01_Core"
 begin
-section ‹Corestriction for top›
+section \<open>Corestriction for top\<close>
 
-theorem corestriction_state [simp]: "S (f ∖⇩p C) = S f"
+theorem corestriction_state [simp]: "S (f \<setminus>\<^sub>p C) = S f"
   by (auto simp: corestrict_p_def S_def corestrict_r_def Field_def)
 
-theorem corestriction_pre [simp]: "Pre (f ∖⇩p C) ⊆ Pre f"
+theorem corestrict_idem: "(p \<setminus>\<^sub>p C) \<setminus>\<^sub>p C = p \<setminus>\<^sub>p C" \<comment> \<open>NEW\<close>
+  by (auto simp: corestrict_p_def S_def Field_def corestrict_r_def)
+
+theorem corestriction_pre [simp]: "Pre (f \<setminus>\<^sub>p C) \<subseteq> Pre f"
   by (auto simp: corestrict_p_def)
 
-theorem corestriction_post [simp]: "post (f ∖⇩p C) ⊆ post f"
+theorem corestriction_post [simp]: "post (f \<setminus>\<^sub>p C) \<subseteq> post f"
   by (auto simp: corestrict_p_def S_def corestrict_r_def Field_def)
 
-lemma corestrict_prop_1: "Range_p (p ∖⇩p D) ⊆ D"
+lemma corestrict_prop_1: "Range_p (p \<setminus>\<^sub>p D) \<subseteq> D"
   by (auto simp: Range_p_def corestrict_p_def corestrict_r_def restrict_r_def)
 
-lemma corestrict_prop_2: "Range_p (p ∖⇩p D) ⊆ Range_p p"
+lemma corestrict_prop_2: "Range_p (p \<setminus>\<^sub>p D) \<subseteq> Range_p p"
   by (auto simp: Range_p_def corestrict_p_def corestrict_r_def restrict_r_def)
 
-theorem corestrict_prop_: "Range_p (p ∖⇩p D) ⊆ Range_p p ∩ D"
+theorem corestrict_prop_: "Range_p (p \<setminus>\<^sub>p D) \<subseteq> Range_p p \<inter> D"
   by (auto simp: Range_p_def corestrict_p_def corestrict_r_def restrict_r_def)
 
-theorem NOT_corestricted_p_refines_p: "p ∖⇩p C ⊆⇩p p"
-  oops ― ‹Not true as corestriction might remove a post relation completely›
+theorem NOT_corestricted_p_refines_p: "p \<setminus>\<^sub>p C \<subseteq>\<^sub>p p"
+  oops \<comment> \<open>Not true as corestriction might remove a post relation completely\<close>
 
-theorem NOT_p_refines_corestricted_p: "p ⊆⇩p p ∖⇩p C"
-  oops ― ‹Not true as corestriction might remove a post ambiguity›
+theorem NOT_p_refines_corestricted_p: "p \<subseteq>\<^sub>p p \<setminus>\<^sub>p C"
+  oops \<comment> \<open>Not true as corestriction might remove a post ambiguity\<close>
 
-theorem corestricted_refines_unrestricted_1: "p ∖⇩p C ⊆⇩p p" ― ‹T31›
+theorem corestricted_refines_unrestricted_1: "p \<setminus>\<^sub>p C \<subseteq>\<^sub>p p" \<comment> \<open>T31\<close>
   oops
-theorem unrestricted_refines_corestricted_1: "p ⊆⇩p p ∖⇩p C"
+theorem unrestricted_refines_corestricted_1: "p \<subseteq>\<^sub>p p \<setminus>\<^sub>p C"
   oops
-theorem corestricted_refines_unrestricted_2: "is_feasible p ⟹ p ∖⇩p C ⊆⇩p p"
+theorem corestricted_refines_unrestricted_2: "is_feasible p \<Longrightarrow> p \<setminus>\<^sub>p C \<subseteq>\<^sub>p p"
   oops
-theorem unrestricted_refines_corestricted_2: "is_feasible p ⟹ p ⊆⇩p p ∖⇩p C"
+theorem unrestricted_refines_corestricted_2: "is_feasible p \<Longrightarrow> p \<subseteq>\<^sub>p p \<setminus>\<^sub>p C"
   oops
 
-theorem corestricted_subprogram_unrestricted: "p ∖⇩p C ≼⇩p p" ― ‹NEW›
+theorem corestricted_subprogram_unrestricted: "p \<setminus>\<^sub>p C \<preceq>\<^sub>p p" \<comment> \<open>NEW\<close>
   by (auto simp: subprogram_def extends_def weakens_def restr_post_def corestrict_p_def corestrict_r_def restrict_r_def S_def Field_def strengthens_def)
 
-theorem unrestricted_weakens_corestricted: "weakens p (p ∖⇩p C)"
+theorem unrestricted_weakens_corestricted: "weakens p (p \<setminus>\<^sub>p C)"
   by (auto simp: weakens_def corestrict_p_def)
 
-theorem corestricted_strengthens_unrestricted: "strengthens (p ∖⇩p C) p"
+theorem corestricted_strengthens_unrestricted: "strengthens (p \<setminus>\<^sub>p C) p"
   by (auto simp: strengthens_def corestrict_p_def restrict_r_def corestrict_r_def)
 
-theorem corestriction_prop: "D ⊆ C ⟹ p ∖⇩p D ⊆⇩p p ∖⇩p C" ― ‹T32›
+theorem corestriction_prop: "D \<subseteq> C \<Longrightarrow> p \<setminus>\<^sub>p D \<subseteq>\<^sub>p p \<setminus>\<^sub>p C" \<comment> \<open>T32\<close>
   oops
 
-theorem corestriction_weakens_prop: "D ⊆ C ⟹ weakens (p ∖⇩p C) (p ∖⇩p D)"
+theorem corestriction_weakens_prop: "D \<subseteq> C \<Longrightarrow> weakens (p \<setminus>\<^sub>p C) (p \<setminus>\<^sub>p D)"
   by (auto simp: weakens_def corestrict_p_def corestrict_r_def)
 
-theorem corestriction_strengthens_prop: "D ⊆ C ⟹ strengthens (p ∖⇩p D) (p ∖⇩p C)"
+theorem corestriction_strengthens_prop: "D \<subseteq> C \<Longrightarrow> strengthens (p \<setminus>\<^sub>p D) (p \<setminus>\<^sub>p C)"
   by (auto simp: strengthens_def corestrict_p_def corestrict_r_def restrict_r_def)
 
-theorem corestriction_subprogram_prop: "D ⊆ C ⟹ (p ∖⇩p D) ≼⇩p (p ∖⇩p C)" ― ‹NEW›
+theorem corestrict_subprogram: "D \<subseteq> C \<Longrightarrow> (p \<setminus>\<^sub>p D) \<preceq>\<^sub>p (p \<setminus>\<^sub>p C)" \<comment> \<open>NEW\<close>
   by (auto simp: corestrict_p_def subprogram_def extends_def corestrict_r_def S_def Field_def weakens_def restr_post_def restrict_r_def strengthens_def)
 
-theorem equivalence_is_maintained_by_corestriction: "f⇩1 ≡⇩p p⇩1 ⟹ (f⇩1 ∖⇩p C) ≡⇩p p⇩1 ∖⇩p C" ― ‹NEW›
+theorem equivalence_is_maintained_by_corestriction: "f\<^sub>1 \<equiv>\<^sub>p p\<^sub>1 \<Longrightarrow> (f\<^sub>1 \<setminus>\<^sub>p C) \<equiv>\<^sub>p p\<^sub>1 \<setminus>\<^sub>p C" \<comment> \<open>NEW\<close>
   by (auto simp: equiv_def restr_post_def restrict_r_def corestrict_p_def corestrict_r_def)
 
-theorem equality_is_maintained_by_corestriction: "f⇩1 ≜ p⇩1 ⟹ (f⇩1 ∖⇩p C) ≜ p⇩1 ∖⇩p C" ― ‹NEW›
+theorem equality_is_maintained_by_corestriction: "f\<^sub>1 \<triangleq> p\<^sub>1 \<Longrightarrow> (f\<^sub>1 \<setminus>\<^sub>p C) \<triangleq> p\<^sub>1 \<setminus>\<^sub>p C" \<comment> \<open>NEW\<close>
   by (auto simp: equal_def corestrict_p_def)
 
-theorem corestrict_feasible: "is_feasible p ⟹ is_feasible (p ∖⇩p C)"
+theorem corestrict_feasible: "is_feasible p \<Longrightarrow> is_feasible (p \<setminus>\<^sub>p C)"
   by (auto simp: is_feasible_def corestrict_p_def)
-theorem refinement_safety_corestriction: "q ⊆⇩p p ⟹ q ∖⇩p C ⊆⇩p p ∖⇩p C" ― ‹T22›
+theorem refinement_safety_corestriction: "q \<subseteq>\<^sub>p p \<Longrightarrow> q \<setminus>\<^sub>p C \<subseteq>\<^sub>p p \<setminus>\<^sub>p C" \<comment> \<open>T22\<close>
   oops
-theorem weakens_corestriction_1: "all_feasible [p, q] ⟹ q ⊆⇩p p ⟹ weakens (q ∖⇩p C) (p ∖⇩p C)" ― ‹T22›
+theorem weakens_corestriction_1: "all_feasible [p, q] \<Longrightarrow> q \<subseteq>\<^sub>p p \<Longrightarrow> weakens (q \<setminus>\<^sub>p C) (p \<setminus>\<^sub>p C)" \<comment> \<open>T22\<close>
   oops
-theorem weakens_corestriction_2: "q ⊆⇩p p ⟹ weakens (p ∖⇩p C) (q ∖⇩p C)" ― ‹T22›
+theorem weakens_corestriction_2: "q \<subseteq>\<^sub>p p \<Longrightarrow> weakens (p \<setminus>\<^sub>p C) (q \<setminus>\<^sub>p C)" \<comment> \<open>T22\<close>
   oops
-theorem strengthens_corestriction_1: "q ⊆⇩p p ⟹ strengthens (p ∖⇩p C) (q ∖⇩p C)" ― ‹T22›
+theorem strengthens_corestriction_1: "q \<subseteq>\<^sub>p p \<Longrightarrow> strengthens (p \<setminus>\<^sub>p C) (q \<setminus>\<^sub>p C)" \<comment> \<open>T22\<close>
   oops
-theorem strengthens_corestriction_2: "q ⊆⇩p p ⟹ strengthens (q ∖⇩p C) (p ∖⇩p C)" ― ‹T22›
+theorem strengthens_corestriction_2: "q \<subseteq>\<^sub>p p \<Longrightarrow> strengthens (q \<setminus>\<^sub>p C) (p \<setminus>\<^sub>p C)" \<comment> \<open>T22\<close>
   by (auto simp: strengthens_def refines_def corestrict_p_def restrict_r_def corestrict_r_def)
 
-theorem corestrict_is_subprogram: "p∖⇩p C ≼⇩p p"
+theorem corestrict_is_subprogram: "p\<setminus>\<^sub>p C \<preceq>\<^sub>p p"
   by (auto simp: subprogram_def extends_def weakens_def strengthens_def corestrict_p_def corestrict_r_def restrict_r_def S_def Field_def)
+
+theorem corestrict_range_prop: "x \<in> C \<Longrightarrow> x \<notin> Range_p (p \<setminus>\<^sub>p C) \<Longrightarrow> x \<notin> Range_p (p)"
+  by (auto simp: Range_p_def corestrict_p_def corestrict_r_def restrict_r_def Range_iff Domain_iff)
+
+theorem corestrict_range_prop_2: "is_feasible a \<Longrightarrow> Range_p a \<subseteq> C \<Longrightarrow> a \<setminus>\<^sub>p C \<equiv>\<^sub>p a"
+  apply (auto simp: is_feasible_def Range_p_def corestrict_p_def equiv_def corestrict_r_def restrict_r_def Domain_iff Range_iff subset_iff restr_post_def)
+  apply fastforce
+  by fastforce
 
 end
