Isabelle/02_Fundamental_operations/Unsafe_composition.thy
@@ -8,8 +8,8 @@ theorem unsafe_composition_state [simp]: "S (p\<^sub>1 ;\<^sub>p p\<^sub>2) = S 
 
 theorem unsafe_compose_assoc [simp]: "(p\<^sub>1 ;\<^sub>p p\<^sub>2) ;\<^sub>p p\<^sub>3 = p\<^sub>1 ;\<^sub>p (p\<^sub>2 ;\<^sub>p p\<^sub>3)" \<comment> \<open>T8\<close>
 proof -
-  have compose_assoc_S: "S (p\<^sub>1 ;\<^sub>p (p\<^sub>2 ;\<^sub>p p\<^sub>3)) = S ((p\<^sub>1 ;\<^sub>p p\<^sub>2) ;\<^sub>p p\<^sub>3)"
-    by (simp add: sup_assoc)
+  have compose_assoc_S: "State (p\<^sub>1 ;\<^sub>p (p\<^sub>2 ;\<^sub>p p\<^sub>3)) = State ((p\<^sub>1 ;\<^sub>p p\<^sub>2) ;\<^sub>p p\<^sub>3)"
+    by (metis Program.select_convs(1) sup_assoc unsafe_composition_def unsafe_composition_state)
 
   have compose_assoc_pre: "Pre (p\<^sub>1 ;\<^sub>p (p\<^sub>2 ;\<^sub>p p\<^sub>3)) = Pre ((p\<^sub>1 ;\<^sub>p p\<^sub>2) ;\<^sub>p p\<^sub>3)"
     by (simp add: unsafe_composition_def)
@@ -28,8 +28,8 @@ proof -
         by (auto simp: compose_assoc_post_1 compose_assoc_post_2)
     qed
 
-  show ?thesis
-    by (metis compose_assoc_S compose_assoc_post select_convs(2) select_convs(3) unsafe_composition_def unsafe_composition_state)
+  from compose_assoc_S compose_assoc_pre compose_assoc_post show ?thesis
+    by fastforce
 qed
 
 theorem unsafe_compose_assoc_2 [simp]: "(p\<^sub>1 ;\<^sub>p p\<^sub>2) ;\<^sub>p p\<^sub>3 \<triangleq> p\<^sub>1 ;\<^sub>p (p\<^sub>2 ;\<^sub>p p\<^sub>3)" \<comment> \<open>T8\<close>
@@ -38,54 +38,54 @@ theorem unsafe_compose_assoc_2 [simp]: "(p\<^sub>1 ;\<^sub>p p\<^sub>2) ;\<^sub>
 theorem unsafe_compose_assoc_3 [simp]: "(p\<^sub>1 ;\<^sub>p p\<^sub>2) ;\<^sub>p p\<^sub>3 \<equiv>\<^sub>p p\<^sub>1 ;\<^sub>p (p\<^sub>2 ;\<^sub>p p\<^sub>3)" \<comment> \<open>T8\<close>
   by (simp add: equals_equiv_relation_3)
 
-theorem equivalence_is_maintained_by_unsafe_composition: "f⇩1 ≡⇩p p⇩1 ⟹ f⇩2 ≡⇩p p⇩2 ⟹ f⇩1 ;⇩p f⇩2 ≡⇩p p⇩1 ;⇩p p⇩2" ― ‹NEW›
+theorem equivalence_is_maintained_by_unsafe_composition: "f\<^sub>1 \<equiv>\<^sub>p p\<^sub>1 \<Longrightarrow> f\<^sub>2 \<equiv>\<^sub>p p\<^sub>2 \<Longrightarrow> f\<^sub>1 ;\<^sub>p f\<^sub>2 \<equiv>\<^sub>p p\<^sub>1 ;\<^sub>p p\<^sub>2" \<comment> \<open>NEW\<close>
   apply (auto simp: equiv_def restr_post_def restrict_r_def unsafe_composition_def corestrict_r_def)
   using mem_Collect_eq relcomp.relcompI snd_conv apply fastforce
   using mem_Collect_eq relcomp.relcompI snd_conv by fastforce
 
-theorem equality_is_maintained_by_unsafe_composition: "f⇩1 ≜ p⇩1 ⟹ f⇩2 ≜ p⇩2 ⟹ f⇩1 ;⇩p f⇩2 ≜ p⇩1 ;⇩p p⇩2" ― ‹NEW›
+theorem equality_is_maintained_by_unsafe_composition: "f\<^sub>1 \<triangleq> p\<^sub>1 \<Longrightarrow> f\<^sub>2 \<triangleq> p\<^sub>2 \<Longrightarrow> f\<^sub>1 ;\<^sub>p f\<^sub>2 \<triangleq> p\<^sub>1 ;\<^sub>p p\<^sub>2" \<comment> \<open>NEW\<close>
   by (auto simp: equal_def restr_post_def unsafe_composition_def)
 
-theorem unsafe_compose_feasible_1: "is_feasible (p⇩1 ;⇩p p⇩2) ⟹ is_feasible p⇩1"
+theorem unsafe_compose_feasible_1: "is_feasible (p\<^sub>1 ;\<^sub>p p\<^sub>2) \<Longrightarrow> is_feasible p\<^sub>1"
   by (auto simp: unsafe_composition_def is_feasible_def corestrict_r_def)
 
-theorem unsafe_compose_feasible_2: "all_feasible [p⇩1, p⇩2] ⟹ Range_p p⇩1 ⊆ Pre p⇩2 ⟹ is_feasible (p⇩1 ;⇩p p⇩2)"
+theorem unsafe_compose_feasible_2: "all_feasible [p\<^sub>1, p\<^sub>2] \<Longrightarrow> Range_p p\<^sub>1 \<subseteq> Pre p\<^sub>2 \<Longrightarrow> is_feasible (p\<^sub>1 ;\<^sub>p p\<^sub>2)"
 proof -
-  assume a1: "all_feasible [p⇩1, p⇩2]"
-  assume a2: "Range_p p⇩1 ⊆ Pre p⇩2"
-  have l1: "Pre (p⇩1 ;⇩p p⇩2) = {a. ∃c. (a,c) ∈ post p⇩1 ∧ a ∈ Pre p⇩1 ∧ c ∈ Pre p⇩2}"
+  assume a1: "all_feasible [p\<^sub>1, p\<^sub>2]"
+  assume a2: "Range_p p\<^sub>1 \<subseteq> Pre p\<^sub>2"
+  have l1: "Pre (p\<^sub>1 ;\<^sub>p p\<^sub>2) = {a. \<exists>c. (a,c) \<in> post p\<^sub>1 \<and> a \<in> Pre p\<^sub>1 \<and> c \<in> Pre p\<^sub>2}"
     using a1 a2 apply (auto simp: unsafe_composition_def is_feasible_def Range_p_def restrict_r_def)
     proof -
       fix x :: 'a
-      assume a1_1: "Range {r ∈ post p⇩1. fst r ∈ Pre p⇩1} ⊆ Pre p⇩2"
-      assume a1_2: "Pre p⇩1 ⊆ Domain (post p⇩1)"
-      assume a1_3: "x ∈ Pre p⇩1"
-      then have "x ∈ Domain (post p⇩1)"
+      assume a1_1: "Range {r \<in> post p\<^sub>1. fst r \<in> Pre p\<^sub>1} \<subseteq> Pre p\<^sub>2"
+      assume a1_2: "Pre p\<^sub>1 \<subseteq> Domain (post p\<^sub>1)"
+      assume a1_3: "x \<in> Pre p\<^sub>1"
+      then have "x \<in> Domain (post p\<^sub>1)"
         using a1_2 by force
-      then have l1_1: "x ∈ Domain {p ∈ post p⇩1. fst p ∈ Pre p⇩1}"
+      then have l1_1: "x \<in> Domain {p \<in> post p\<^sub>1. fst p \<in> Pre p\<^sub>1}"
         using a1_3 by fastforce
-      have "Range {p ∈ post p⇩1. fst p ∈ Pre p⇩1} ⊆ Pre p⇩2"
-        using a1_1 by (smt (z3))
-      then show "∃a. (x, a) ∈ post p⇩1 ∧ a ∈ Pre p⇩2"
+      have "Range {p \<in> post p\<^sub>1. fst p \<in> Pre p\<^sub>1} \<subseteq> Pre p\<^sub>2"
+        using a1_1 by auto
+      then show "\<exists>a. (x, a) \<in> post p\<^sub>1 \<and> a \<in> Pre p\<^sub>2"
         using l1_1 by blast
     qed
-  have l2: "Domain (post (p⇩1 ;⇩p p⇩2)) = {a. ∃c. (a,c) ∈ post p⇩1 ∧ c ∈ Pre p⇩2}"
+  have l2: "Domain (post (p\<^sub>1 ;\<^sub>p p\<^sub>2)) = {a. \<exists>c. (a,c) \<in> post p\<^sub>1 \<and> c \<in> Pre p\<^sub>2}"
     proof -
-      have l2_1: "post (p⇩1 ;⇩p p⇩2) = {(a,b). ∃c. (a,c) ∈ post p⇩1 ∧ (c,b) ∈ post p⇩2 ∧ c ∈ Pre p⇩2}"
+      have l2_1: "post (p\<^sub>1 ;\<^sub>p p\<^sub>2) = {(a,b). \<exists>c. (a,c) \<in> post p\<^sub>1 \<and> (c,b) \<in> post p\<^sub>2 \<and> c \<in> Pre p\<^sub>2}"
         using a1 a2 by (auto simp: Range_p_def is_feasible_def unsafe_composition_def restr_post_def restrict_r_def)
-      then have l2_2: "Domain (post (p⇩1 ;⇩p p⇩2)) = {a. ∃b c. (a,c) ∈ post p⇩1 ∧ (c,b) ∈ post p⇩2 ∧ c ∈ Pre p⇩2}"
+      then have l2_2: "Domain (post (p\<^sub>1 ;\<^sub>p p\<^sub>2)) = {a. \<exists>b c. (a,c) \<in> post p\<^sub>1 \<and> (c,b) \<in> post p\<^sub>2 \<and> c \<in> Pre p\<^sub>2}"
         using a1 a2 by (auto simp: l2_1)
-      then show "Domain (post (p⇩1 ;⇩p p⇩2)) = {a. ∃c. (a,c) ∈ post p⇩1 ∧ c ∈ Pre p⇩2}"
+      then show "Domain (post (p\<^sub>1 ;\<^sub>p p\<^sub>2)) = {a. \<exists>c. (a,c) \<in> post p\<^sub>1 \<and> c \<in> Pre p\<^sub>2}"
         apply (auto simp: l2_2)
         using a1 a2 l2_1 apply auto[1]
         using a1 a2 apply (auto simp: is_feasible_def)
-        by (smt (verit, del_insts) Domain.cases a1 l2_2 mem_Collect_eq subsetD)
+        by (meson Domain_iff subsetD)
     qed
-  have l3: "{a. ∃c. (a,c) ∈ post p⇩1 ∧ a ∈ Pre p⇩1 ∧ c ∈ Pre p⇩2} ⊆ {a. ∃c. (a,c) ∈ post p⇩1 ∧ c ∈ Pre p⇩2}"
+  have l3: "{a. \<exists>c. (a,c) \<in> post p\<^sub>1 \<and> a \<in> Pre p\<^sub>1 \<and> c \<in> Pre p\<^sub>2} \<subseteq> {a. \<exists>c. (a,c) \<in> post p\<^sub>1 \<and> c \<in> Pre p\<^sub>2}"
     by auto
-  have l4: "Pre (p⇩1 ;⇩p p⇩2) ⊆  Domain (post (p⇩1 ;⇩p p⇩2))"
+  have l4: "Pre (p\<^sub>1 ;\<^sub>p p\<^sub>2) \<subseteq>  Domain (post (p\<^sub>1 ;\<^sub>p p\<^sub>2))"
     using a1 a2 l1 l2 by auto
-  show "is_feasible (p⇩1 ;⇩p p⇩2)"
+  show "is_feasible (p\<^sub>1 ;\<^sub>p p\<^sub>2)"
     by (simp add: is_feasible_def l4)
 qed
 
