Isabelle/04_Composed_operations/If_then_else.thy
@@ -6,7 +6,7 @@ section \<open>If then else for top.\<close>
 lemma ite_S: "S (ITE C q\<^sub>1 q\<^sub>2) = S q\<^sub>1 \<union> S q\<^sub>2"
   by (auto simp: if_then_else_def S_def restrict_p_def restrict_r_def Field_def choice_def restr_post_def)
 
-theorem property_on_ite_1: "ITE C p\<^sub>1 p\<^sub>2 = ITE (-C) p\<^sub>2 p\<^sub>1" \<comment> \<open>T52, T57\<close>
+theorem cond_swap: "ITE C p\<^sub>1 p\<^sub>2 = ITE (-C) p\<^sub>2 p\<^sub>1" \<comment> \<open>Cond_swap\<close>
   by (auto simp: if_then_else_def choice_def)
 
 value "ITE {1::nat} 
@@ -18,7 +18,7 @@ value "\<lparr>State={}, Pre = {1::nat, 2}, post = {(1,2), (2,1)}\<rparr> \<ssla
 theorem property_on_ite_2: "Pre (p \<sslash>\<^sub>p C) = Pre (ITE C p (Skip (S p)))" \<comment> \<open>T53\<close>
   oops
 
-theorem refinement_safety_ite: "q\<^sub>1 \<subseteq>\<^sub>p p\<^sub>1 \<Longrightarrow> q\<^sub>2 \<subseteq>\<^sub>p p\<^sub>2 \<Longrightarrow> ITE C q\<^sub>1 q\<^sub>2 \<subseteq>\<^sub>p ITE C p\<^sub>1 p\<^sub>2" \<comment> \<open>T51\<close>
+theorem cond_refine3: "q\<^sub>1 \<subseteq>\<^sub>p p\<^sub>1 \<Longrightarrow> q\<^sub>2 \<subseteq>\<^sub>p p\<^sub>2 \<Longrightarrow> ITE C q\<^sub>1 q\<^sub>2 \<subseteq>\<^sub>p ITE C p\<^sub>1 p\<^sub>2" \<comment> \<open>Cond_refine3\<close>
   apply (auto simp: refines_def)
   apply (auto simp: extends_def ite_S) [1]
   apply (auto simp: weakens_def if_then_else_def restrict_p_def restrict_r_def choice_def S_def) [1]
@@ -26,6 +26,7 @@ theorem refinement_safety_ite: "q\<^sub>1 \<subseteq>\<^sub>p p\<^sub>1 \<Longri
 
 
 theorem ite_commutative: "ITE C p\<^sub>1 p\<^sub>2 = ITE (-C) p\<^sub>2 p\<^sub>1"
+  by (auto simp: if_then_else_def)
 
 
 
