Isabelle/T_04_Composed_operations.thy
@@ -6,7 +6,6 @@ theory T_04_Composed_operations
 "04_Composed_operations/Big_choice"
 "04_Composed_operations/Complex_operation_interactions"
 "04_Composed_operations/Fixed_repetition"
-"04_Composed_operations/Fixed_repetition_support"
 "04_Composed_operations/Guarded_conditional"
 "04_Composed_operations/If_then_else"
 "04_Composed_operations/Non_atomic_concurrency"
