Isabelle/T_05_Properties.thy
@@ -1,6 +1,7 @@
 theory T_05_Properties
   imports 
 "T_04_Composed_operations"
+"05_Properties/Contract"
 "05_Properties/Invariant"
 "05_Properties/Loop_invariant"
 begin
